Batteries/Data/Iterators.lean
@@ -1,2 +1,3 @@
 module
 public import Batteries.Data.Iterators.Scan
+public import Batteries.Data.Iterators.Lemmas
