Batteries/Data/Iterators/Lemmas/Scan.lean
@@ -1,0 +1,63 @@
+module
+prelude
+public import Batteries.Data.Iterators.Scan
+public import Batteries.Data.List.Scan
+
+public section
+
+
+namespace Std.Iterators
+
+private abbrev IterM.toScanIterM [Iterator α Id β] [Monad m] [MonadLiftT Id m]
+    (it : IterM (α := α) Id β) (f : γ → β → m γ) (acc : γ) (emittedInit : Bool := false) : IterM (α := ScanM α Id m β γ f) m γ :=
+  toIterM ⟨it.internalState, acc, emittedInit⟩ m γ
+
+private theorem toList_scanM_emittedTrue [Iterator α Id β] [Finite α Id] [Monad m] [LawfulMonad m]
+  [IteratorCollect α Id Id (β := β)] [LawfulIteratorCollect α Id Id (β := β)]
+  {f : γ → β → m γ} {acc : γ} {it : IterM (α := α) Id β} 
+  : (toIterM (m := m) (β := γ) (⟨it.internalState, acc, true⟩ : ScanM α Id m β γ f)).toList 
+    = (return (← List.scanlM f acc (← it.toList)).tail) 
+  := by
+    induction it using IterM.inductSteps generalizing acc
+    rename_i it ihy ihs
+    repeat rw [IterM.toList_eq_match_step]
+    simp_all [ScanM.instIterator, IterM.step, Iterator.step]
+    apply bind_congr
+    intro step
+    match hstep : step.inflate with
+    | ⟨.yield inner' out, hp⟩ =>
+      simp_all [liftM, monadLift, Id.run, toIterM, Functor.map]
+      apply bind_congr
+      intro a
+      rw [ihy hp, ← List.scanlM_cons_head_tail]
+      simp
+    | ⟨.skip inner', hp⟩ =>
+      simp_all [liftM, monadLift, Id.run, toIterM];
+    | ⟨.done, hp⟩ =>
+      simp_all
+
+
+@[local simp ←]
+private theorem toIterM_eq_mk {state : ScanM α m n β γ f} :
+    (toIterM state n γ : IterM n γ) = { internalState := state } := rfl
+
+
+private theorem toList_scanM_emittedFalse [Iterator α Id β] [Finite α Id] [Monad m] [LawfulMonad m]
+    [IteratorCollect α Id Id (β := β)] [LawfulIteratorCollect α Id Id (β := β)]
+    {f : γ → β → m γ} {acc : γ} {it : IterM (α := α) Id β} :
+    (toIterM (⟨it.internalState, acc, false⟩ : ScanM α Id m β γ f) m γ).toList = 
+    List.scanlM f acc it.toList := by
+  rw [IterM.toList_eq_match_step]
+  simp only [Iterator.step, ScanM.instIterator, IterM.step]
+  simp_all [liftM, monadLift, Id.run, toList_scanM_emittedTrue]
+  rw [← List.scanlM_cons_head_tail f acc it.toList]
+  simp
+
+theorem IterM.toList_scanM [Iterator α Id β] [Finite α Id] [Monad m] [LawfulMonad m]
+    [IteratorCollect α Id Id (β := β)] [LawfulIteratorCollect α Id Id (β := β)]
+    {f : γ → β → m γ} {init : γ} (it : IterM (α := α) Id β) :
+    (it.scanM f init).toList = List.scanlM f init it.toList := by
+  simp only [IterM.scanM]
+  rw [toList_scanM_emittedFalse]
+
+end Std.Iterators
