Batteries/Data/List/Scan.lean
@@ -296,6 +296,13 @@ theorem scanrM_eq_scanlM_reverse [Monad m] [LawfulMonad m] {f : α → β → m 
   unfold flip
   unfold flip at h
   simp_all
+
+theorem scanlM_cons_head_tail [Monad m] [LawfulMonad m] (f : γ → β → m γ) (init : γ) (xs : List β) :
+    (return (init :: (← List.scanlM f init xs).tail)) = List.scanlM f init xs := by 
+  induction xs generalizing init <;> simp_all
+
+  
+
 /-! ### partialSums/partialProd -/
 
 @[simp, grind =]
